src/program_proof/tulip/paxos/res.v
@@ -1,6 +1,7 @@
 From Perennial.program_proof Require Import grove_prelude.
+From Perennial.program_proof.rsm Require Import big_sep.
 From Perennial.program_proof.rsm.pure Require Import quorum extend list.
-From Perennial.program_proof.tulip.paxos Require Import base.
+From Perennial.program_proof.tulip.paxos Require Import base consistency.
 
 Section res.
   Context `{!paxos_ghostG Σ}.
@@ -98,9 +99,10 @@ Section res.
       own_internal_log γ l2.
     Admitted.
 
-    Lemma internal_log_witness {γ l} :
+    Lemma internal_log_witness {γ l} lb :
+      prefix lb l ->
       own_internal_log γ l -∗
-      is_internal_log_lb γ l.
+      is_internal_log_lb γ lb.
     Admitted.
 
     Lemma internal_log_prefix {γ l lb} :
@@ -115,7 +117,7 @@ Section res.
 
     (** Elements. *)
 
-    Definition own_proposals γ (vs : proposals) : iProp Σ.
+    Definition own_proposals γ (ps : proposals) : iProp Σ.
     Admitted.
 
     Definition own_proposal γ (t : nat) (v : ledger) : iProp Σ.
@@ -133,23 +135,23 @@ Section res.
 
     (** Rules. *)
 
-    Lemma proposal_insert {γ vs} t v :
-      vs !! t = None ->
-      own_proposals γ vs ==∗
-      own_proposals γ (<[t := v]> vs) ∗ own_proposal γ t v.
+    Lemma proposal_insert {γ ps} t v :
+      ps !! t = None ->
+      own_proposals γ ps ==∗
+      own_proposals γ (<[t := v]> ps) ∗ own_proposal γ t v.
     Admitted.
 
-    Lemma proposal_lookup {γ vs t v} :
+    Lemma proposal_lookup {γ ps t v} :
       own_proposal γ t v -∗
-      own_proposals γ vs -∗
-      ⌜vs !! t = Some v⌝.
+      own_proposals γ ps -∗
+      ⌜ps !! t = Some v⌝.
     Admitted.
 
-    Lemma proposal_update {γ vs t v1} v2 :
+    Lemma proposal_update {γ ps t v1} v2 :
       prefix v1 v2 ->
       own_proposal γ t v1 -∗
-      own_proposals γ vs ==∗
-      own_proposal γ t v2 ∗ own_proposals γ (<[t := v2]> vs).
+      own_proposals γ ps ==∗
+      own_proposal γ t v2 ∗ own_proposals γ (<[t := v2]> ps).
     Admitted.
 
     Lemma proposal_witness {γ t v} :
@@ -157,10 +159,10 @@ Section res.
       is_proposal_lb γ t v.
     Admitted.
 
-    Lemma proposal_prefix {γ t vlb v} :
+    Lemma proposal_prefix {γ ps t vlb} :
       is_proposal_lb γ t vlb -∗
-      own_proposal γ t v -∗
-      ⌜prefix vlb v⌝.
+      own_proposals γ ps -∗
+      ∃ v, ⌜ps !! t = Some v ∧ prefix vlb v⌝.
     Admitted.
 
   End proposal.
@@ -169,7 +171,7 @@ Section res.
 
     (** Elements. *)
 
-    Definition own_base_proposals γ (vs : proposals) : iProp Σ.
+    Definition own_base_proposals γ (ps : proposals) : iProp Σ.
     Admitted.
 
     Definition is_base_proposal_receipt γ (t : nat) (v : ledger) : iProp Σ.
@@ -184,16 +186,16 @@ Section res.
 
     (** Rules. *)
 
-    Lemma base_proposal_insert {γ vs} t v :
-      vs !! t = None ->
-      own_base_proposals γ vs ==∗
-      own_base_proposals γ (<[t := v]> vs) ∗ is_base_proposal_receipt γ t v.
+    Lemma base_proposal_insert {γ ps} t v :
+      ps !! t = None ->
+      own_base_proposals γ ps ==∗
+      own_base_proposals γ (<[t := v]> ps) ∗ is_base_proposal_receipt γ t v.
     Admitted.
 
-    Lemma base_proposal_lookup {γ vs t v} :
+    Lemma base_proposal_lookup {γ ps t v} :
       is_base_proposal_receipt γ t v -∗
-      own_base_proposals γ vs -∗
-      ⌜vs !! t = Some v⌝.
+      own_base_proposals γ ps -∗
+      ⌜ps !! t = Some v⌝.
     Admitted.
 
   End base_proposal.
@@ -240,7 +242,7 @@ Section res.
 
     (** Elements. *)
 
-    Definition own_accepted_proposals γ (nid : u64) (vs : proposals) : iProp Σ.
+    Definition own_accepted_proposals γ (nid : u64) (ps : proposals) : iProp Σ.
     Admitted.
 
     Definition own_accepted_proposal γ (nid : u64) (t : nat) (v : ledger) : iProp Σ.
@@ -258,17 +260,23 @@ Section res.
 
     (** Rules. *)
 
-    Lemma accepted_proposal_insert {γ nid vs t v} :
-      vs !! t = None ->
-      own_accepted_proposals γ nid vs ==∗
-      own_accepted_proposals γ nid (<[t := v]> vs) ∗ own_accepted_proposal γ nid t v.
+    Lemma accepted_proposal_insert {γ nid ps t v} :
+      ps !! t = None ->
+      own_accepted_proposals γ nid ps ==∗
+      own_accepted_proposals γ nid (<[t := v]> ps) ∗ own_accepted_proposal γ nid t v.
     Admitted.
 
-    Lemma accepted_proposal_update {γ nid vs t v1} v2 :
+    Lemma accepted_proposal_update {γ nid ps t v1} v2 :
       prefix v1 v2 ->
       own_accepted_proposal γ nid t v1 -∗
-      own_accepted_proposals γ nid vs ==∗
-      own_accepted_proposal γ nid t v2 ∗ own_accepted_proposals γ t (<[t := v2]> vs).
+      own_accepted_proposals γ nid ps ==∗
+      own_accepted_proposal γ nid t v2 ∗ own_accepted_proposals γ t (<[t := v2]> ps).
+    Admitted.
+
+    Lemma accepted_proposal_prefix {γ nid ps t vlb} :
+      is_accepted_proposal_lb γ nid t vlb -∗
+      own_accepted_proposals γ nid ps -∗
+      ∃ v, ⌜ps !! t = Some v ∧ prefix vlb v⌝.
     Admitted.
 
   End accepted_proposal.
@@ -377,46 +385,258 @@ Section inv.
   Definition free_terms_after (t : nat) (ts : gset nat) :=
     ∀ t', (t < t')%nat -> t' ∉ ts.
 
+  Definition prefix_base_ledger γ t v : iProp Σ :=
+    ∃ vlb, is_base_proposal_receipt γ t vlb ∗ ⌜prefix vlb v⌝.
+
+  Definition prefix_growing_ledger γ t v : iProp Σ :=
+    ∃ vub, is_proposal_lb γ t vub ∗ ⌜prefix v vub⌝.
+
   Definition node_inv γ nid terml : iProp Σ :=
     ∃ ds psa termc logn,
-      "Hpastd" ∷ own_past_nodedecs γ nid ds ∗
+      "Hds" ∷ own_past_nodedecs γ nid ds ∗
       "Hpsa"   ∷ own_accepted_proposals γ nid psa ∗
       "Htermc" ∷ own_current_term_half γ nid termc ∗
       "Hterml" ∷ own_ledger_term_half γ nid terml ∗
       "Hlogn"  ∷ own_node_ledger_half γ nid logn ∗
+      "#Hpsalbs" ∷ ([∗ map] t ↦ v ∈ psa, prefix_base_ledger γ t v) ∗
+      "#Hpsaubs" ∷ ([∗ map] t ↦ v ∈ psa, prefix_growing_ledger γ t v) ∗
       "%Hfixed"  ∷ ⌜fixed_proposals ds psa⌝ ∗
       "%Hdompsa" ∷ ⌜free_terms_after terml (dom psa)⌝ ∗
       "%Hlogn"   ∷ ⌜psa !! terml = Some logn⌝ ∗
       "%Hlends"  ∷ ⌜length ds = termc⌝ ∗
       "%Htermlc" ∷ ⌜(terml ≤ termc)%nat⌝.
 
+  Definition node_inv_without_ds_psa
+    γ nid terml (ds : list nodedec) (psa : proposals) : iProp Σ :=
+    ∃ termc logn,
+      "Htermc" ∷ own_current_term_half γ nid termc ∗
+      "Hterml" ∷ own_ledger_term_half γ nid terml ∗
+      "Hlogn"  ∷ own_node_ledger_half γ nid logn ∗
+      "%Hdompsa" ∷ ⌜free_terms_after terml (dom psa)⌝ ∗
+      "%Hlogn"   ∷ ⌜psa !! terml = Some logn⌝ ∗
+      "%Hlends"  ∷ ⌜length ds = termc⌝ ∗
+      "%Htermlc" ∷ ⌜(terml ≤ termc)%nat⌝.
+
+  Definition node_inv_psa γ nid psa : iProp Σ :=
+    "Hpsa"     ∷ own_accepted_proposals γ nid psa ∗
+    "#Hpsalbs" ∷ ([∗ map] t ↦ v ∈ psa, prefix_base_ledger γ t v) ∗
+    "#Hpsaubs" ∷ ([∗ map] t ↦ v ∈ psa, prefix_growing_ledger γ t v).
+
+  Definition node_inv_ds_psa γ nid ds psa : iProp Σ :=
+    "Hpsa"    ∷ node_inv_psa γ nid psa ∗
+    "Hpastd"  ∷ own_past_nodedecs γ nid ds ∗
+    "%Hfixed" ∷ ⌜fixed_proposals ds psa⌝.
+
   Definition prefix_of_accepted_proposal γ nid t logi: iProp Σ :=
     ∃ loga,
       "#Hloga"   ∷ is_accepted_proposal_lb γ nid t loga ∗
       "%Hprefix" ∷ ⌜prefix logi loga⌝.
 
-  Definition safe_internal_log γ nids logi : iProp Σ :=
+  Definition safe_ledger γ nids logi : iProp Σ :=
     ∃ nidsq t,
       "#Hacpt"   ∷ ([∗ set] nid ∈ nidsq, prefix_of_accepted_proposal γ nid t logi) ∗
-      "%Hquorum" ∷ ⌜cquorum_size nids nidsq⌝.
+      "%Hquorum" ∷ ⌜cquorum nids nidsq⌝.
 
-  Definition equal_latest_longest_proposal_nodedec (dsq : gmap u64 (list nodedec)) t v :=
-    equal_latest_longest_proposal_with (mbind nodedec_to_ledger) dsq t v.
+  Definition equal_latest_longest_proposal_nodedec (dssq : gmap u64 (list nodedec)) t v :=
+    equal_latest_longest_proposal_with (mbind nodedec_to_ledger) dssq t v.
 
   Definition safe_base_proposal γ nids t v : iProp Σ :=
-    ∃ dssq,
-      "#Hdsq"    ∷ ([∗ map] nid ↦ ds ∈ dssq, is_past_nodedecs_lb γ nid ds) ∗
-      "%Hlen"    ∷ ⌜map_Forall (λ _ ds, (t ≤ length ds)%nat) dssq⌝ ∗
-      "%Hincl"   ∷ ⌜dom dssq ⊆ nids⌝ ∗
-      "%Hquorum" ∷ ⌜cquorum_size nids (dom dssq)⌝ ∗
-      "%Heq"     ∷ ⌜equal_latest_longest_proposal_nodedec dssq t v⌝.
+    ∃ dssqlb,
+      "#Hdsq"    ∷ ([∗ map] nid ↦ ds ∈ dssqlb, is_past_nodedecs_lb γ nid ds) ∗
+      "%Hlen"    ∷ ⌜map_Forall (λ _ ds, (t ≤ length ds)%nat) dssqlb⌝ ∗
+      "%Hquorum" ∷ ⌜cquorum nids (dom dssqlb)⌝ ∗
+      "%Heq"     ∷ ⌜equal_latest_longest_proposal_nodedec dssqlb t v⌝.
 
   Definition latest_term_before_nodedec t (ds : list nodedec) :=
     latest_term_before_with (mbind nodedec_to_ledger) t ds.
 
+  Lemma latest_term_before_nodedec_unfold t ds :
+    latest_term_before_nodedec t ds = latest_term_before_with (mbind nodedec_to_ledger) t ds.
+  Proof. done. Qed.
+
   Definition latest_term_nodedec ds :=
     latest_term_before_nodedec (length ds) ds.
 
+  Lemma latest_term_before_nodedec_app t ds dsapp :
+    (t ≤ length ds)%nat ->
+    latest_term_before_nodedec t (ds ++ dsapp) = latest_term_before_nodedec t ds.
+  Proof.
+    intros Hlen.
+    rewrite /latest_term_before_nodedec.
+    induction t as [| t IH]; first done.
+    rewrite /= -IH; last lia.
+    by rewrite lookup_app_l; last lia.
+  Qed.
+
+  Lemma latest_term_nodedec_snoc_Reject ds :
+    latest_term_nodedec (ds ++ [Reject]) = latest_term_nodedec ds.
+  Proof.
+    rewrite /latest_term_nodedec /latest_term_before_nodedec last_length /=.
+    rewrite lookup_snoc_length /=.
+    by apply latest_term_before_nodedec_app.
+  Qed.
+
+  Lemma latest_term_nodedec_extend_Reject t ds :
+    latest_term_nodedec (extend t Reject ds) = latest_term_nodedec ds.
+  Proof.
+    unfold extend.
+    induction t as [| t IH]; first by rewrite app_nil_r.
+    destruct (decide (t < length ds)%nat) as [Hlt | Hge].
+    { replace (t - length ds)%nat with O in IH by lia.
+      by replace (S t - length ds)%nat with O by lia.
+    }
+    replace (S t - length ds)%nat with (S (t - length ds)%nat) by lia.
+    by rewrite replicate_S_end assoc latest_term_nodedec_snoc_Reject.
+  Qed.
+
+  Lemma fixed_proposals_latest_term_before_nodedec ds psa t :
+    (t ≤ length ds)%nat ->
+    fixed_proposals ds psa ->
+    latest_term_before_nodedec t ds = latest_term_before t psa.
+  Proof.
+    intros Hlen Hfixed.
+    rewrite /latest_term_before_nodedec /latest_term_before.
+    induction t as [| p IH]; first done.
+    simpl.
+    assert (p < length ds)%nat as Hp by lia.
+    apply list_lookup_lt in Hp as [d Hd].
+    specialize (Hfixed _ _ Hd).
+    rewrite Hd /= -Hfixed IH; [done | lia].
+  Qed.
+
+  Definition latest_term_before_quorum_nodedec (dss : gmap u64 (list nodedec)) t :=
+    latest_term_before_quorum_with (mbind nodedec_to_ledger) dss t.
+
+  Lemma latest_term_before_quorum_nodedec_unfold dss t :
+    latest_term_before_quorum_nodedec dss t =
+    latest_term_before_quorum_with (mbind nodedec_to_ledger) dss t.
+  Proof. done. Qed.
+
+  Lemma latest_term_before_quorum_nodedec_prefixes dss dsslb t :
+    map_Forall2 (λ _ dslb ds, prefix dslb ds ∧ (t ≤ length dslb)%nat) dsslb dss ->
+    latest_term_before_quorum_nodedec dsslb t = latest_term_before_quorum_nodedec dss t.
+  Proof.
+    intros Hprefixes.
+    rewrite /latest_term_before_quorum_nodedec /latest_term_before_quorum_with.
+    f_equal.
+    apply map_eq.
+    intros nid.
+    rewrite 2!lookup_fmap.
+    specialize (Hprefixes nid).
+    destruct (dsslb !! nid) as [dslb |], (dss !! nid) as [ds |]; [| done | done | done].
+    simpl. simpl in Hprefixes.
+    f_equal.
+    destruct Hprefixes as [[dsapp ->] Hlen].
+    by rewrite -2!latest_term_before_nodedec_unfold latest_term_before_nodedec_app.
+  Qed.
+
+  Lemma fixed_proposals_latest_term_before_quorum_nodedec dss (bs : gmap u64 proposals) t :
+    map_Forall2 (λ _ ds psa, fixed_proposals ds psa ∧ (t ≤ length ds)%nat) dss bs ->
+    latest_term_before_quorum_nodedec dss t = latest_term_before_quorum bs t.
+  Proof.
+    intros Hfixed.
+    rewrite /latest_term_before_quorum_nodedec /latest_term_before_quorum.
+    rewrite /latest_term_before_quorum_with.
+    f_equal.
+    apply map_eq.
+    intros x.
+    rewrite 2!lookup_fmap.
+    specialize (Hfixed x).
+    destruct (dss !! x) as [ds |], (bs !! x) as [ps |]; [| done | done | done].
+    simpl.
+    f_equal.
+    destruct Hfixed as [Hfixed Hlen].
+    by apply fixed_proposals_latest_term_before_nodedec.
+  Qed.
+
+  Definition ledger_in_term_nodedec t (ds : list nodedec) :=
+    ledger_in_term_with (mbind nodedec_to_ledger) t ds.
+
+  Lemma fixed_proposals_ledger_in_term_nodedec ds psa t :
+    (t < length ds)%nat ->
+    fixed_proposals ds psa ->
+    ledger_in_term_nodedec t ds = ledger_in_term t psa.
+  Proof.
+    intros Hlen Hfixed.
+    rewrite /ledger_in_term_nodedec /ledger_in_term /ledger_in_term_with /=.
+    apply list_lookup_lt in Hlen as [d Hd].
+    specialize (Hfixed _ _ Hd).
+    by rewrite Hd Hfixed.
+  Qed.
+
+  Definition longest_proposal_in_term_nodedec (dss : gmap u64 (list nodedec)) t :=
+    longest_proposal_in_term_with (mbind nodedec_to_ledger) dss t.
+
+  Lemma longest_proposal_in_term_nodedec_unfold dss t :
+    longest_proposal_in_term_nodedec dss t =
+    longest_proposal_in_term_with (mbind nodedec_to_ledger) dss t.
+  Proof. done. Qed.
+
+  Lemma longest_proposal_in_term_nodedec_prefixes dss dsslb t :
+    map_Forall2 (λ _ dslb ds, prefix dslb ds ∧ (t < length dslb)%nat) dsslb dss ->
+    longest_proposal_in_term_nodedec dsslb t = longest_proposal_in_term_nodedec dss t.
+  Proof.
+    intros Hprefixes.
+    rewrite /longest_proposal_in_term_nodedec /longest_proposal_in_term_with.
+    f_equal.
+    apply map_eq.
+    intros nid.
+    rewrite 2!lookup_fmap.
+    specialize (Hprefixes nid).
+    rewrite /ledger_in_term_with.
+    destruct (dsslb !! nid) as [dslb |], (dss !! nid) as [ds |]; [| done | done | done].
+    simpl. simpl in Hprefixes.
+    f_equal.
+    destruct Hprefixes as [Hprefix Hlen].
+    by rewrite (prefix_lookup_lt _ _ _ Hlen Hprefix).
+  Qed.
+
+  Lemma fixed_proposals_longest_proposal_in_term_nodedec dss (bs : gmap u64 proposals) t :
+    map_Forall2 (λ _ ds psa, fixed_proposals ds psa ∧ (t < length ds)%nat) dss bs ->
+    longest_proposal_in_term_nodedec dss t = longest_proposal_in_term bs t.
+  Proof.
+    intros Hfixed.
+    rewrite /longest_proposal_in_term_nodedec /longest_proposal_in_term.
+    rewrite /longest_proposal_in_term_with.
+    f_equal.
+    apply map_eq.
+    intros x.
+    rewrite 2!lookup_fmap.
+    specialize (Hfixed x).
+    destruct (dss !! x) as [ds |], (bs !! x) as [ps |]; [| done | done | done].
+    simpl.
+    f_equal.
+    destruct Hfixed as [Hfixed Hlen].
+    by apply fixed_proposals_ledger_in_term_nodedec.
+  Qed.
+
+  Lemma fixed_proposals_equal_latest_longest_proposal_nodedec dss bs t v :
+    map_Forall2 (λ _ ds psa, fixed_proposals ds psa ∧ (t ≤ length ds)%nat) dss bs ->
+    equal_latest_longest_proposal_nodedec dss t v ->
+    equal_latest_longest_proposal bs t v.
+  Proof.
+    rewrite /equal_latest_longest_proposal /equal_latest_longest_proposal_nodedec.
+    rewrite /equal_latest_longest_proposal_with.
+    intros Hfixed Heq.
+    case_decide as Hv; first done.
+    rewrite -Heq -latest_term_before_quorum_nodedec_unfold.
+    rewrite (fixed_proposals_latest_term_before_quorum_nodedec _ _ _ Hfixed).
+    set t' := latest_term_before_quorum _ _.
+    rewrite -longest_proposal_in_term_nodedec_unfold.
+    unshelve erewrite (fixed_proposals_longest_proposal_in_term_nodedec dss bs t' _).
+    { intros nid.
+      specialize (Hfixed nid).
+      destruct (dss !! nid) as [ds |], (bs !! nid) as [ps |]; [| done | done | done].
+      simpl. simpl in Hfixed.
+      destruct Hfixed as [Hfixed Hlen].
+      split; first done.
+      subst t'.
+      eapply Nat.lt_le_trans; last apply Hlen.
+      by apply latest_term_before_quorum_with_lt.
+    }
+    done.
+  Qed.
+  
   Definition past_nodedecs_latest_before γ nid ds termc terml v : iProp Σ :=
     "#Hpastd"  ∷ is_past_nodedecs_lb γ nid ds ∗
     "%Hlends"  ∷ ⌜(termc ≤ length ds)%nat⌝ ∗
@@ -436,9 +656,9 @@ Section inv.
       "Hnodes" ∷ ([∗ map] nid ↦ terml ∈ termlm, node_inv γ nid terml) ∗
       (* TODO: constraints between internal and external states *)
       (* constraints on internal states *)
-      "#Hsafelogi"  ∷ safe_internal_log γ nids logi ∗
+      "#Hsafelogi"  ∷ safe_ledger γ nids logi ∗
       "#Hsafepsb"   ∷ ([∗ map] t ↦ v ∈ psb, safe_base_proposal γ nids t v) ∗
-      "%Hbase"      ∷ ⌜map_Forall2 (λ _ (vlb v : ledger), prefix vlb v) psb ps⌝ ∗
+      "%Hvp"        ∷ ⌜valid_proposals ps psb⌝ ∗
       "%Hdomtermlm" ∷ ⌜dom termlm = nids⌝ ∗
       "%Hdompsb"    ∷ ⌜free_terms (dom psb) termlm⌝.
 
@@ -457,7 +677,8 @@ End inv.
  * - ascend(t, v): insert [(t, v)] into [proposals] and [base_proposals].
  * - extend(t, v): update [proposals !! t] to [v]
  * - prepare(t): snoc [accepted_proposals !! (length ballot)] to [ballot] if it exists, and extend [ballot] with [Reject] up to [t].
- * - accept(t, v): insert/update [(t, v)] to [accepted_proposals].
+ * - advance(t, v): insert [(t, v)] into [accepted_proposals].
+ * - accept(t, v): update [accepted_proposals !! t] to [v].
  * - commit(v): update [internal_log] to [v].
  *)
 
@@ -523,38 +744,6 @@ Section prepare.
     by rewrite Hfree.
   Qed.
 
-  Lemma latest_term_before_nodedec_append t ds dsapp :
-    (t ≤ length ds)%nat ->
-    latest_term_before_nodedec t (ds ++ dsapp) = latest_term_before_nodedec t ds.
-  Proof.
-    intros Hlen.
-    rewrite /latest_term_before_nodedec.
-    induction t as [| t IH]; first done.
-    rewrite /= -IH; last lia.
-    by rewrite lookup_app_l; last lia.
-  Qed.
-
-  Lemma latest_term_nodedec_snoc_Reject ds :
-    latest_term_nodedec (ds ++ [Reject]) = latest_term_nodedec ds.
-  Proof.
-    rewrite /latest_term_nodedec /latest_term_before_nodedec last_length /=.
-    rewrite lookup_snoc_length /=.
-    by apply latest_term_before_nodedec_append.
-  Qed.
-
-  Lemma latest_term_nodedec_extend_Reject t ds :
-    latest_term_nodedec (extend t Reject ds) = latest_term_nodedec ds.
-  Proof.
-    unfold extend.
-    induction t as [| t IH]; first by rewrite app_nil_r.
-    destruct (decide (t < length ds)%nat) as [Hlt | Hge].
-    { replace (t - length ds)%nat with O in IH by lia.
-      by replace (S t - length ds)%nat with O by lia.
-    }
-    replace (S t - length ds)%nat with (S (t - length ds)%nat) by lia.
-    by rewrite replicate_S_end assoc latest_term_nodedec_snoc_Reject.
-  Qed.
-
   Lemma latest_term_nodedec_snoc_Accept ds v :
     latest_term_nodedec (ds ++ [Accept v]) = length ds.
     rewrite /latest_term_nodedec /latest_term_before_nodedec last_length /= lookup_app_r; last done.
@@ -579,21 +768,6 @@ Section prepare.
     by rewrite Hfree (IH Ht1).
   Qed.
 
-  Lemma fixed_proposals_latest_term_before_nodedec ds psa t :
-    (t ≤ length ds)%nat ->
-    fixed_proposals ds psa ->
-    latest_term_before_nodedec t ds = latest_term_before t psa.
-  Proof.
-    intros Hlen Hfixed.
-    rewrite /latest_term_before_nodedec /latest_term_before /=.
-    induction t as [| p IH]; first done.
-    simpl.
-    assert (p < length ds)%nat as Hp by lia.
-    apply list_lookup_lt in Hp as [d Hd].
-    specialize (Hfixed _ _ Hd).
-    rewrite Hd /= -Hfixed IH; [done | lia].
-  Qed.
-
   Lemma node_inv_prepare γ nid termc termc' terml v :
     (termc < termc')%nat ->
     own_current_term_half γ nid termc -∗
@@ -614,10 +788,10 @@ Section prepare.
       iMod (current_term_update termc' with "HtermcX Htermc") as "[HtermcX Htermc]".
       (* Extend the node decisions [d] with [Reject]. *)
       set ds' := extend termc' Reject ds.
-      iMod (past_nodedecs_update ds' with "Hpastd") as "Hpastd".
+      iMod (past_nodedecs_update ds' with "Hds") as "Hds".
       { apply extend_prefix. }
       (* Extract a witness of the extended past decision. *)
-      iDestruct (past_nodedecs_witness with "Hpastd") as "#Hdlb".
+      iDestruct (past_nodedecs_witness with "Hds") as "#Hdlb".
       (* Re-establish [fixed_proposals d' psa]. *)
       unshelve epose proof
         (fixed_proposals_inv_prepare_term_lt _ termc' _ ds _ Hdompsa Hfixed) as Hfixed'.
@@ -649,12 +823,12 @@ Section prepare.
     iMod (current_term_update termc' with "HtermcX Htermc") as "[HtermcX Htermc]".
     (* Snoc [Accept v] and extend the node decisions [d] with [Reject]. *)
     set ds' := extend termc' Reject (ds ++ [Accept v]).
-    iMod (past_nodedecs_update ds' with "Hpastd") as "Hpastd".
+    iMod (past_nodedecs_update ds' with "Hds") as "Hds".
     { etrans; last apply extend_prefix.
       by apply prefix_app_r.
     }
     (* Extract a witness of the extended past decision. *)
-    iDestruct (past_nodedecs_witness with "Hpastd") as "#Hdlb".
+    iDestruct (past_nodedecs_witness with "Hds") as "#Hdlb".
     unshelve epose proof
       (fixed_proposals_inv_prepare_term_eq _ _ _ _ _ Hlends Hlt Hlogn Hdompsa Hfixed) as Hfixed'.
     iFrame "∗ # %".
@@ -708,3 +882,320 @@ Section prepare.
   Qed.
 
 End prepare.
+
+Section commit.
+  Context `{!paxos_ghostG Σ}.
+
+  Lemma equal_latest_longest_proposal_nodedec_prefix dss dsslb t v :
+    map_Forall2 (λ _ dslb ds, prefix dslb ds ∧ (t ≤ length dslb)%nat) dsslb dss ->
+    equal_latest_longest_proposal_nodedec dsslb t v ->
+    equal_latest_longest_proposal_nodedec dss t v.
+  Proof.
+    rewrite /equal_latest_longest_proposal_nodedec /equal_latest_longest_proposal_with.
+    rewrite -2!latest_term_before_quorum_nodedec_unfold.
+    rewrite -2!longest_proposal_in_term_nodedec_unfold.
+    intros Hprefixes Heq.
+    case_decide as Ht; first done.
+    rewrite -(latest_term_before_quorum_nodedec_prefixes _ _ _ Hprefixes).
+    set t' := (latest_term_before_quorum_nodedec _ _) in Heq *.
+    assert (Hlt : (t' < t)%nat).
+    { by apply latest_term_before_quorum_with_lt. }
+    rewrite -(longest_proposal_in_term_nodedec_prefixes dss dsslb); first apply Heq.
+    apply (map_Forall2_impl _ _ _ _ Hprefixes).
+    intros _ dslb ds [Hprefix Hlen].
+    split; [done | lia].
+  Qed.
+
+  Lemma nodes_inv_impl_valid_base_proposals γ nids bs psb dss :
+    dom bs = nids ->
+    ([∗ map] t ↦ v ∈ psb, safe_base_proposal γ nids t v) -∗
+    ([∗ map] nid ↦ ds; psa ∈ dss; bs, node_inv_ds_psa γ nid ds psa) -∗
+    ⌜valid_base_proposals bs psb⌝.
+  Proof.
+    iIntros (Hdombs) "Hsafe Hinv".
+    iIntros (t v Hv).
+    iDestruct (big_sepM_lookup with "Hsafe") as "Hsafe"; first apply Hv.
+    iNamed "Hsafe".
+    rewrite /valid_base_proposal.
+    rewrite big_sepM2_alt.
+    iDestruct "Hinv" as "[%Hdomdss Hinv]".
+    iDestruct (big_sepM_dom_subseteq_difference _ _ (dom dssqlb) with "Hinv") as "Hm".
+    { rewrite dom_map_zip_with_L Hdomdss intersection_idemp Hdombs.
+      by destruct Hquorum as [Hincl _].
+    }
+    iDestruct "Hm" as (m [Hdomm Hinclm]) "[Hm _]".
+    set dssq := fst <$> m.
+    set bsq := snd <$> m.
+    iExists bsq.
+    iAssert (⌜map_Forall2 (λ _ dslb ds, prefix dslb ds ∧ (t ≤ length dslb)%nat) dssqlb dssq⌝)%I
+      as %Hprefix.
+    { iIntros (x).
+      destruct (dssqlb !! x) as [dslb |] eqn:Hdslb, (dssq !! x) as [ds |] eqn:Hds; last first.
+      { done. }
+      { rewrite -not_elem_of_dom -Hdomm not_elem_of_dom in Hdslb.
+        subst dssq.
+        by rewrite lookup_fmap Hdslb /= in Hds.
+      }
+      { subst dssq.
+        by rewrite -not_elem_of_dom dom_fmap_L Hdomm not_elem_of_dom Hdslb in Hds.
+      }
+      simpl.
+      iDestruct (big_sepM_lookup with "Hdsq") as "Hdsqx"; first apply Hdslb.
+      rewrite lookup_fmap_Some in Hds.
+      destruct Hds as ([ds' psa] & Hds & Hmx). simpl in Hds. subst ds'.
+      iDestruct (big_sepM_lookup with "Hm") as "Hinv"; first apply Hmx.
+      iNamed "Hinv". simpl.
+      iDestruct (past_nodedecs_prefix with "Hdsqx Hpastd") as %Hprefix.
+      by specialize (Hlen _ _ Hdslb).
+    }
+    pose proof (equal_latest_longest_proposal_nodedec_prefix _ _ _ _ Hprefix Heq) as Heq'.
+    iAssert (⌜map_Forall2 (λ _ ds psa, fixed_proposals ds psa ∧ (t ≤ length ds)%nat) dssq bsq⌝)%I
+      as %Hfixed.
+    { iIntros (x).
+      destruct (dssq !! x) as [ds |] eqn:Hds, (bsq !! x) as [psa |] eqn:Hpsa; last first.
+      { done. }
+      { rewrite -not_elem_of_dom dom_fmap_L in Hds.
+        apply elem_of_dom_2 in Hpsa.
+        by rewrite dom_fmap_L in Hpsa.
+      }
+      { rewrite -not_elem_of_dom dom_fmap_L in Hpsa.
+        apply elem_of_dom_2 in Hds.
+        by rewrite dom_fmap_L in Hds.
+      }
+      simpl.
+      iDestruct (big_sepM_lookup _ _ x (ds, psa) with "Hm") as "Hinv".
+      { rewrite lookup_fmap_Some in Hds.
+        destruct Hds as ([ds1 psa1] & Hds & Hmx1). simpl in Hds. subst ds1.
+        rewrite lookup_fmap_Some in Hpsa.
+        destruct Hpsa as ([ds2 psa2] & Hpsa & Hmx2). simpl in Hpsa. subst psa2.
+        rewrite Hmx1 in Hmx2.
+        by inv Hmx2.
+      }
+      iNamed "Hinv".
+      specialize (Hprefix x).
+      assert (is_Some (dssqlb !! x)) as [dslb Hdslb].
+      { rewrite -elem_of_dom -Hdomm elem_of_dom.
+        apply lookup_fmap_Some in Hds as (dp & _ & Hinv).
+        done.
+      }
+      rewrite Hds Hdslb /= in Hprefix.
+      iPureIntro.
+      split; first apply Hfixed.
+      destruct Hprefix as [Hprefix Hlelen].
+      apply prefix_length in Hprefix.
+      lia.
+    }
+    iPureIntro.
+    split.
+    { subst bsq.
+      trans (snd <$> map_zip dss bs).
+      { by apply map_fmap_mono. }
+      rewrite snd_map_zip; first done.
+      intros x Hbsx.
+      by rewrite -elem_of_dom -Hdomdss elem_of_dom in Hbsx.
+    }
+    split.
+    { subst bsq.
+      rewrite dom_fmap_L Hdomm Hdombs.
+      by destruct Hquorum as [_ Hquorum].
+    }
+    by eapply fixed_proposals_equal_latest_longest_proposal_nodedec.
+  Qed.
+
+  Lemma nodes_inv_impl_valid_lb_ballots γ bs psb :
+    own_base_proposals γ psb -∗
+    ([∗ map] nid ↦ psa ∈ bs, node_inv_psa γ nid psa) -∗
+    ⌜valid_lb_ballots bs psb⌝.
+  Proof.
+    iIntros "Hpsb Hinv".
+    iIntros (nid psa Hpsa).
+    iDestruct (big_sepM_lookup with "Hinv") as "Hinv"; first apply Hpsa.
+    iNamed "Hinv".
+    iIntros (t v Hv).
+    iDestruct (big_sepM_lookup with "Hpsalbs") as (vlb) "[Hvlb %Hprefix]"; first apply Hv.
+    iDestruct (base_proposal_lookup with "Hvlb Hpsb") as %Hvlb.
+    by eauto.
+  Qed.
+
+  Lemma nodes_inv_impl_valid_ub_ballots γ bs ps :
+    own_proposals γ ps -∗
+    ([∗ map] nid ↦ psa ∈ bs, node_inv_psa γ nid psa) -∗
+    ⌜valid_ub_ballots bs ps⌝.
+  Proof.
+    iIntros "Hps Hinv".
+    iIntros (nid psa Hpsa).
+    iDestruct (big_sepM_lookup with "Hinv") as "Hinv"; first apply Hpsa.
+    iNamed "Hinv".
+    iIntros (t v Hv).
+    iDestruct (big_sepM_lookup with "Hpsaubs") as (vlb) "[Hvub %Hprefix]"; first apply Hv.
+    iDestruct (proposal_prefix with "Hvub Hps") as %(vub & Hvub & Hprefixvlb).
+    iPureIntro.
+    exists vub.
+    split; first apply Hvub.
+    by trans vlb.
+  Qed.
+
+  Lemma node_inv_extract_ds_psa γ nid terml :
+    node_inv γ nid terml -∗
+    ∃ ds psa, node_inv_without_ds_psa γ nid terml ds psa ∗
+              node_inv_ds_psa γ nid ds psa.
+  Proof. iIntros "Hinv". iNamed "Hinv". iFrame "∗ # %". Qed.
+
+  Lemma nodes_inv_extract_ds_psa γ termlm :
+    ([∗ map] nid ↦ terml ∈ termlm, node_inv γ nid terml) -∗
+    ∃ dss bs, ([∗ map] nid ↦ terml; dp ∈ termlm; map_zip dss bs,
+                 node_inv_without_ds_psa γ nid terml dp.1 dp.2) ∗
+              ([∗ map] nid ↦ ds; psa ∈ dss; bs, node_inv_ds_psa γ nid ds psa).
+  Proof.
+    iIntros "Hinvs".
+    set Φ := (λ nid terml dp,
+                node_inv_without_ds_psa γ nid terml dp.1 dp.2 ∗
+                node_inv_ds_psa γ nid dp.1 dp.2)%I.
+    iDestruct (big_sepM_sepM2_exists Φ termlm with "[Hinvs]") as (dpm) "Hdpm".
+    { iApply (big_sepM_mono with "Hinvs").
+      iIntros (nid terml Hterml) "Hinv".
+      subst Φ.
+      iNamed "Hinv".
+      iExists (ds, psa).
+      iFrame "∗ # %".
+    }
+    iDestruct (big_sepM2_dom with "Hdpm") as %Hdom.
+    subst Φ.
+    iNamed "Hdpm".
+    iDestruct (big_sepM2_sep with "Hdpm") as "[Hinv Hdp]".
+    iExists (fst <$> dpm), (snd <$> dpm).
+    rewrite map_zip_fst_snd.
+    iFrame "Hinv".
+    iDestruct (big_sepM2_flip with "Hdp") as "Hdp".
+    rewrite -big_sepM_big_sepM2; last apply Hdom.
+    rewrite big_sepM2_alt map_zip_fst_snd.
+    iFrame "Hdp".
+    iPureIntro.
+    by rewrite 2!dom_fmap_L.
+  Qed.
+
+  Lemma nodes_inv_merge_ds_psa γ termlm dss bs :
+    ([∗ map] nid ↦ terml; dp ∈ termlm; map_zip dss bs,
+       node_inv_without_ds_psa γ nid terml dp.1 dp.2) -∗
+    ([∗ map] nid ↦ ds; psa ∈ dss; bs, node_inv_ds_psa γ nid ds psa) -∗
+    ([∗ map] nid ↦ terml ∈ termlm, node_inv γ nid terml).
+  Proof.
+    iIntros "Hinv Hdp".
+    iDestruct (big_sepM2_alt with "Hdp") as "[%Hdom Hdp]".
+    iDestruct (big_sepM2_dom with "Hinv") as %Hdomtermlm.
+    iDestruct (big_sepM_big_sepM2_1 with "Hdp") as "Hdp".
+    { apply Hdomtermlm. }
+    rewrite big_sepM2_flip.
+    iCombine "Hinv Hdp" as "Hinv".
+    rewrite -big_sepM2_sep.
+    iApply (big_sepM2_sepM_impl with "Hinv").
+    { apply Hdomtermlm. }
+    iIntros (nid dp terml terml' Hdp Hterml Hterml') "!> [Hinv Hdp]".
+    rewrite Hterml in Hterml'. symmetry in Hterml'. inv Hterml'.
+    iNamed "Hinv".
+    iNamed "Hdp".
+    iNamed "Hpsa".
+    iFrame "∗ # %".
+  Qed.
+
+  Lemma nodes_inv_safe_ledger_impl_chosen γ nids bs v :
+    dom bs = nids ->
+    ([∗ map] nid ↦ psa ∈ bs, node_inv_psa γ nid psa) -∗
+    safe_ledger γ nids v -∗
+    ⌜chosen bs v⌝.
+  Proof.
+    iIntros (Hdombs) "Hinv Hv".
+    iNamed "Hv".
+    set bsq := (filter (λ x, x.1 ∈ nidsq) bs).
+    iExists t, bsq.
+    rewrite base.and_assoc.
+    iSplit.
+    { iPureIntro.
+      split; first apply map_filter_subseteq.
+      rewrite Hdombs.
+      subst bsq.
+      destruct Hquorum as [Hincl Hquorum].
+      rewrite (dom_filter_L _ _ nidsq); first apply Hquorum.
+      intros nid.
+      split; last by intros (ps & _ & Hin).
+      intros Hin.
+      assert (is_Some (bs !! nid)) as [ps Hps].
+      { rewrite -elem_of_dom Hdombs. set_solver. }
+      by exists ps.
+    }
+    iIntros (nid ps Hps).
+    iDestruct (big_sepS_elem_of _ _ nid with "Hacpt") as "Hprefix".
+    { by apply map_lookup_filter_Some_1_2 in Hps. }
+    iNamed "Hprefix".
+    iDestruct (big_sepM_lookup _ _ nid with "Hinv") as "Hnid".
+    { eapply lookup_weaken; [apply Hps | apply map_filter_subseteq]. }
+    iNamed "Hnid".
+    iDestruct (accepted_proposal_prefix with "Hloga Hpsa") as %(va & Hva & Hprefixva).
+    iPureIntro.
+    exists va.
+    split; first apply Hva.
+    by trans loga.
+  Qed.
+
+  Lemma nodes_inv_ds_psa_impl_nodes_inv_psa γ dss bs :
+    ([∗ map] nid ↦ ds; psa ∈ dss; bs, node_inv_ds_psa γ nid ds psa) -∗
+    ([∗ map] nid ↦ psa ∈ bs, node_inv_psa γ nid psa). 
+  Proof.
+    iIntros "Hpds".
+    rewrite big_sepM2_flip.
+    iApply (big_sepM2_sepM_impl with "Hpds"); first done.
+    iIntros (nid psa ds psa' Hpsa Hds Hpsa') "!> Hpd".
+    rewrite Hpsa in Hpsa'. symmetry in Hpsa'. inv Hpsa'.
+    by iNamed "Hpd".
+  Qed.
+
+  Lemma paxos_inv_commit γ nids logi' :
+    safe_ledger γ nids logi' -∗
+    paxos_inv γ nids ==∗
+    paxos_inv γ nids ∗
+    is_internal_log_lb γ logi'.
+  Proof.
+    iIntros "#Hsafe Hinv".
+    iNamed "Hinv".
+    (* Extract past decisions and accepted proposals from the node invariant. *)
+    iDestruct (nodes_inv_extract_ds_psa with "Hnodes") as (dss bs) "[Hnodes Hpds]".
+    iDestruct (big_sepM2_dom with "Hpds") as %Hdompds.
+    iDestruct (big_sepM2_dom with "Hnodes") as %Hdombs.
+    rewrite dom_map_zip_with_L Hdompds Hdomtermlm in Hdombs. symmetry in Hdombs.
+    replace (_ ∩ _) with (dom bs) in Hdombs by set_solver.
+    (* not sure why the following fails, so using replace above as a workaround *)
+    (* rewrite intersection_idemp in Hdombs. *)
+    (* Obtain [valid_base_proposals bs psb]. *)
+    iDestruct (nodes_inv_impl_valid_base_proposals with "Hsafepsb Hpds") as %Hvbp.
+    { apply Hdombs. }
+    (* Obtain [nodes_inv_valid_lb_ballots bs psb]. *)
+    iDestruct (nodes_inv_impl_valid_lb_ballots _ bs with "Hpsb [Hpds]") as %Hvlb.
+    { by iApply nodes_inv_ds_psa_impl_nodes_inv_psa. }
+    (* Obtain [nodes_inv_valid_ub_ballots bs ps]. *)
+    iDestruct (nodes_inv_impl_valid_ub_ballots _ bs with "Hps [Hpds]") as %Hvub.
+    { by iApply nodes_inv_ds_psa_impl_nodes_inv_psa. }
+    (* Finally, derive [consistency bs]. *)
+    pose proof (vlb_vub_vbp_vp_impl_consistency _ _ _ Hvlb Hvub Hvbp Hvp) as Hcst.
+    (* Now, derive [chosen bs logi] and [chosen bs logi']. *)
+    iDestruct (nodes_inv_safe_ledger_impl_chosen _ _ bs with "[Hpds] Hsafelogi") as %Hchosen.
+    { apply Hdombs. }
+    { by iApply nodes_inv_ds_psa_impl_nodes_inv_psa. }
+    iDestruct (nodes_inv_safe_ledger_impl_chosen _ _ bs with "[Hpds] Hsafe") as %Hchosen'.
+    { apply Hdombs. }
+    { by iApply nodes_inv_ds_psa_impl_nodes_inv_psa. }
+    (* Derive [prefix logi logi' ∨ prefix logi' logi]. *)
+    specialize (Hcst _ _ Hchosen Hchosen').
+    (* Merge [node_inv_ds_psa] back. *)
+    iDestruct (nodes_inv_merge_ds_psa with "Hnodes Hpds") as "Hnodes".
+    destruct Hcst as [Hge | Hle]; last first.
+    { (* Case: The old log is at least as long as the new log. Simply extract a witness. *)
+      iDestruct (internal_log_witness logi' with "Hlogi") as "#Hlb"; first apply Hle.
+      by iFrame "∗ # %".
+    }
+    (* Case: The new log is at least as long as the old log. Update the log. *)
+    iMod (internal_log_update with "Hlogi") as "Hlogi"; first apply Hge.
+    iDestruct (internal_log_witness logi' with "Hlogi") as "#Hlb"; first done.
+    by iFrame "∗ # %".
+  Qed.
+
+End commit.
